WIP: multiple return values

SSA/Core/Framework.lean
@@ -66,39 +66,40 @@ theorem _root_.Pure.pure_cast {f} [inst : Pure f] (b : β) (h : β = α) :
 
 /- # Classes -/
 
-abbrev RegionSignature Ty := List (Ctxt Ty × Ty)
+abbrev RegionSignature Ty := List (Ctxt Ty × List Ty)
 
 structure Signature (Ty : Type) where
   mkEffectful ::
-  sig        : List Ty
-  regSig     : RegionSignature Ty
-  outTy      : Ty
-  effectKind : EffectKind := .pure
+  sig         : List Ty
+  regSig      : RegionSignature Ty
+  returnTypes : List Ty
+  effectKind  : EffectKind := .pure
 
-abbrev Signature.mk (sig : List Ty) (regSig : RegionSignature Ty) (outTy : Ty) : Signature Ty :=
- { sig := sig, regSig := regSig, outTy := outTy }
+abbrev Signature.mk (sig : List Ty) (regSig : RegionSignature Ty) (returnTypes : List Ty) : Signature Ty :=
+ { sig, regSig, returnTypes }
 
 class DialectSignature (d : Dialect) where
   signature : d.Op → Signature d.Ty
 export DialectSignature (signature)
 
-section
+namespace DialectSignature
 variable {d} [s : DialectSignature d]
 
-def DialectSignature.sig        := Signature.sig ∘ s.signature
-def DialectSignature.regSig     := Signature.regSig ∘ s.signature
-def DialectSignature.outTy      := Signature.outTy ∘ s.signature
-def DialectSignature.effectKind := Signature.effectKind ∘ s.signature
+def sig          := Signature.sig ∘ s.signature
+def regSig       := Signature.regSig ∘ s.signature
+def returnTypes  := Signature.returnTypes ∘ s.signature
+def effectKind   := Signature.effectKind ∘ s.signature
 
-end
-
+end DialectSignature
 
 class DialectDenote (d : Dialect) [TyDenote d.Ty] [DialectSignature d] where
   denote : (op : d.Op) → HVector toType (DialectSignature.sig op) →
-    (HVector (fun t : Ctxt d.Ty × d.Ty => t.1.Valuation
-      → EffectKind.impure.toMonad d.m (toType t.2))
+    (HVector (fun t : Ctxt d.Ty × List d.Ty =>
+      t.1.Valuation
+      → EffectKind.impure.toMonad d.m (HVector toType t.2))
             (DialectSignature.regSig op)) →
-    ((DialectSignature.effectKind op).toMonad d.m (toType <| DialectSignature.outTy op))
+    ((DialectSignature.effectKind op).toMonad d.m
+      (HVector toType <| DialectSignature.returnTypes op))
 
 /-
 Some considerations about purity:
@@ -143,33 +144,38 @@ impurely.
 -/
 
 
+
 /- # Datastructures -/
 section DataStructures
 
 variable (d : Dialect) [DialectSignature d]
 
 mutual
-/-- An intrinsically typed expression whose effect is *at most* EffectKind -/
-inductive Expr : (Γ : Ctxt d.Ty) → (eff : EffectKind) → (ty : d.Ty) → Type where
-  | mk {Γ} {ty} (op : d.Op)
-    (ty_eq : ty = DialectSignature.outTy op)
+/-- `Expr Γ_in eff Γ_out` represents an intrinsically typed expression whose
+effect is *at most* EffectKind.
+
+Note that `Γ_in` is the context under which the expression is (intrinsically)
+well-typed, and `Γ_out` is the context *after* the expression, i.e., with any
+new variables added. -/
+inductive Expr : (Γ_in : Ctxt d.Ty) → (eff : EffectKind) → (Γ_out : Ctxt d.Ty) → Type where
+  | mk {Γ_in Γ_out : Ctxt _} (op : d.Op)
+    (ty_eq : Γ_out = Γ_in ++ DialectSignature.returnTypes op)
     (eff_le : DialectSignature.effectKind op ≤ eff)
-    (args : HVector (Var Γ) <| DialectSignature.sig op)
+    (args : HVector (Var Γ_in) <| DialectSignature.sig op)
     /- For now, assume that regions are impure.
        We keep it this way to minimize the total amount of disruption in our definitions.
        We shall change this once the rest of the file goes through. -/
-    (regArgs : HVector (fun t : Ctxt d.Ty × d.Ty => Com t.1 .impure t.2)
-      (DialectSignature.regSig op)) : Expr Γ eff ty
-
+    (regArgs : HVector (fun t : Ctxt d.Ty × List d.Ty => Com t.1 .impure t.2)
+      (DialectSignature.regSig op)) : Expr Γ_in eff Γ_out
 
 /-- A very simple intrinsically typed program: a sequence of let bindings.
 Note that the `EffectKind` is uniform: if a `Com` is `pure`, then the expression
 and its body are pure, and if a `Com` is `impure`, then both the expression and
 the body are impure!
 -/
-inductive Com : Ctxt d.Ty → EffectKind → d.Ty → Type where
-  | ret {eff : EffectKind} (v : Var Γ t) : Com Γ eff t
-  | var (e : Expr Γ eff α) (body : Com (Γ.snoc α) eff β) : Com Γ eff β
+inductive Com : Ctxt d.Ty → EffectKind → List d.Ty → Type where
+  | ret {eff : EffectKind} (vs : HVector Γ.Var tys) : Com Γ eff tys
+  | var (e : Expr Γ eff Δ) (body : Com Δ eff β) : Com Γ eff β
 end
 
 /-- `Lets d Γ_in Γ_out` is a sequence of lets which are well-formed under
@@ -177,7 +183,7 @@ context `Γ_out` and result in context `Γ_in`. -/
 inductive Lets (Γ_in : Ctxt d.Ty) (eff : EffectKind) :
     (Γ_out : Ctxt d.Ty) → Type where
   | nil : Lets Γ_in eff Γ_in
-  | var (body : Lets Γ_in eff Γ_out) (e : Expr d Γ_out eff t) : Lets Γ_in eff (Γ_out.snoc t)
+  | var (body : Lets Γ_in eff Γ_out) (e : Expr d Γ_out eff Δ) : Lets Γ_in eff Δ
 
 /-- `Zipper d Γ_in eff Γ_mid ty` represents a particular position in a program, by storing the
 `Lets` that come before this position separately from the `Com` that represents the rest.
@@ -186,13 +192,11 @@ current position.
 
 While technically the position is in between two let-bindings, by convention we say that the first
 binding of `top : Lets ..` is the current binding of a particular zipper. -/
-structure Zipper (Γ_in : Ctxt d.Ty) (eff : EffectKind) (Γ_mid : Ctxt d.Ty) (ty : d.Ty) where
+structure Zipper (Γ_in : Ctxt d.Ty) (eff : EffectKind) (Γ_mid : Ctxt d.Ty) (tys : List d.Ty) where
   /-- The let-bindings at the top of the zipper -/
   top : Lets d Γ_in eff Γ_mid
   /-- The program at the bottom of the zipper -/
-  bot : Com d Γ_mid eff ty
-
-
+  bot : Com d Γ_mid eff tys
 
 /-! ### Repr instance -/
 section Repr
@@ -229,7 +233,7 @@ private def formatFormalArgListTuple [Repr Ty] (ts : List Ty) : Format :=
 
 mutual
   /-- Convert a HVector of region arguments into a List of format strings. -/
-  partial def reprRegArgsAux [Repr d.Ty] {ts : List (Ctxt d.Ty × d.Ty)}
+  partial def reprRegArgsAux [Repr d.Ty] {ts : RegionSignature d.Ty}
     (regArgs : HVector (fun t => Com d t.1 EffectKind.impure t.2) ts) : List Format :=
     match ts with
     | [] => []
@@ -242,10 +246,10 @@ mutual
 
   partial def Expr.repr (_ : Nat) : Expr d Γ eff t → Format
     | ⟨op, _, _, args, regArgs⟩ =>
-        let outTy := DialectSignature.outTy op
+        let returnTypes := DialectSignature.returnTypes op
         let argTys := DialectSignature.sig op
         let regArgs := Format.parenIfNonempty " (" ")" Format.line (reprRegArgsAux regArgs)
-        f!"{repr op}{formatArgTuple args}{regArgs} : {formatTypeTuple argTys} → ({repr outTy})"
+        f!"{repr op}{formatArgTuple args}{regArgs} : {formatTypeTuple argTys} → ({repr returnTypes})"
 
   /-- Format string for a Com, with the region parentheses and formal argument list. -/
   partial def Com.repr (prec : Nat) (com : Com d Γ eff t) : Format :=
@@ -295,9 +299,9 @@ their types, and the resulting output type.
 -/
 partial def Expr.toString [ToString d.Op] : Expr d Γ eff t → String
   | Expr.mk (op : d.Op) _ _ args _regArgs =>
-    let outTy : d.Ty := DialectSignature.outTy op
+    let returnTypes := DialectSignature.returnTypes op
     let argTys := DialectSignature.sig op
-    s!"{ToString.toString op}{formatArgTuple args} : {formatTypeTupleToString argTys} -> ({ToString.toString outTy})"
+    s!"{ToString.toString op}{formatArgTuple args} : {formatTypeTupleToString argTys} -> ({ToString.toString returnTypes})"
 
 /-- This function recursivly converts the body of a `Com` into its string representation.
 Each bound variable is printed with its index and corresponding expression. -/
@@ -326,7 +330,7 @@ mutual -- DecEq
 variable {d} [DialectSignature d]
 
 protected instance HVector.decidableEqReg [DecidableEq d.Op] [DecidableEq d.Ty] :
-    ∀ {l : List (Ctxt d.Ty × d.Ty)}, DecidableEq (HVector (fun t => Com d t.1 .impure t.2) l)
+    ∀ {l : RegionSignature d.Ty}, DecidableEq (HVector (fun t => Com d t.1 .impure t.2) l)
   | _, .nil, .nil => isTrue rfl
   | _, .cons x₁ v₁, .cons x₂ v₂ =>
     letI := HVector.decidableEqReg v₁ v₂
@@ -334,7 +338,7 @@ protected instance HVector.decidableEqReg [DecidableEq d.Op] [DecidableEq d.Ty] 
     decidable_of_iff (x₁ = x₂ ∧ v₁ = v₂) (by simp)
 
 protected instance Expr.decidableEq [DecidableEq d.Op] [DecidableEq d.Ty] :
-    {Γ : Ctxt d.Ty} → {ty : d.Ty} → DecidableEq (Expr d Γ eff ty)
+    {Γ Δ : Ctxt d.Ty} → DecidableEq (Expr d Γ eff Δ)
   | _, _, .mk op₁ rfl eff_le₁ arg₁ regArgs₁, .mk op₂ eq eff_le₂ arg₂ regArgs₂ =>
     if ho : op₁ = op₂
     then by
@@ -345,10 +349,10 @@ protected instance Expr.decidableEq [DecidableEq d.Op] [DecidableEq d.Ty] :
     else isFalse (by simp_all)
 
 protected instance Com.decidableEq [DecidableEq d.Op] [DecidableEq d.Ty]
-    {Γ : Ctxt d.Ty} {eff : EffectKind} {ty : d.Ty} : DecidableEq (Com d Γ eff ty)
+    {Γ : Ctxt d.Ty} {eff : EffectKind} {tys : List d.Ty} : DecidableEq (Com d Γ eff tys)
   | .ret v₁, .ret v₂ => decidable_of_iff (v₁ = v₂) (by simp)
-  | .var (α := α₁) e₁ body₁, .var (α := α₂) e₂ body₂ =>
-    if hα : α₁ = α₂
+  | .var (Δ := Δ₁) e₁ body₁, .var (Δ := Δ₂) e₂ body₂ =>
+    if hα : Δ₁ = Δ₂
     then by
       subst hα
       letI := Expr.decidableEq e₁ e₂
@@ -369,10 +373,11 @@ end DataStructures
 variable {d : Dialect} [DialectSignature d]
 
 @[elab_as_elim]
-def Com.recAux' {motive : ∀ {Γ eff t}, Com d Γ eff t → Sort u}
-    (ret : ∀ {Γ t} {eff : EffectKind}, (v : Var Γ t) → motive (eff := eff) (Com.ret v))
-    (var : ∀ {Γ} {t u : d.Ty} {eff},
-      (e : Expr d Γ eff t) → (body : Com d (Ctxt.snoc Γ t) eff u) →
+def Com.recAux' {motive : ∀ {Γ eff ts}, Com d Γ eff ts → Sort u}
+    (ret : ∀ {Γ : Ctxt _} {ts} {eff : EffectKind},
+      (vs : HVector Γ.Var ts) → motive (eff := eff) (Com.ret vs))
+    (var : ∀ {Γ Δ} {ts : List d.Ty} {eff},
+      (e : Expr d Γ eff Δ) → (body : Com d Δ eff ts) →
         motive body → motive (Com.var e body)) :
     ∀ {Γ eff t}, (com : Com d Γ eff t) → motive com
   | _, _, _, Com.ret v => ret v
@@ -382,9 +387,9 @@ def Com.recAux' {motive : ∀ {Γ eff t}, Com d Γ eff t → Sort u}
 -- ^^^^ `Com.rec` is noncomputable, so have a computable version as well
 --      See `Com.recAux'_eq` for a theorem that states these definitions are equal
 def Com.rec' {motive : ∀ {Γ eff t}, Com d Γ eff t → Sort u}
-    (ret : ∀ {Γ t} {eff : EffectKind}, (v : Var Γ t) → motive (eff := eff) (Com.ret v))
-    (var : ∀ {Γ} {t u : d.Ty} {eff},
-      (e : Expr d Γ eff t) → (body : Com d (Ctxt.snoc Γ t) eff u) →
+    (ret : ∀ {Γ : Ctxt _} {ts} {eff : EffectKind}, (vs : HVector Γ.Var ts) → motive (eff := eff) (Com.ret vs))
+    (var : ∀ {Γ Δ} {ts : List d.Ty} {eff},
+      (e : Expr d Γ eff Δ) → (body : Com d Δ eff ts) →
         motive body → motive (Com.var e body)) :
     ∀ {Γ eff t}, (com : Com d Γ eff t) → motive com :=
   /- HACK: the obvious definition of `rec'` using the match compiler does not have the
@@ -395,11 +400,11 @@ def Com.rec' {motive : ∀ {Γ eff t}, Com d Γ eff t → Sort u}
     (fun e body _ r => var e body r) -- `Com.var` case
     ⟨⟩ (fun _ _ _ _ => ⟨⟩)
 
-@[simp] lemma Com.rec'_ret (v : Var Γ t) {motive eff} {ret var} :
-    (Com.ret (d:=d) (eff := eff) v).rec' (motive:=motive) ret var = ret v :=
+@[simp] lemma Com.rec'_ret {Γ : Ctxt _} {vs : HVector Γ.Var t} {motive eff} {ret var} :
+    (Com.ret (d:=d) (eff := eff) vs).rec' (motive:=motive) ret var = ret vs :=
   rfl
 
-@[simp] lemma Com.rec'_var (e : Expr d Γ eff t) (body : Com d _ _ u)
+@[simp] lemma Com.rec'_var (e : Expr d Γ eff Δ) (body : Com d Δ eff ts)
     {motive} {ret var} :
     (Com.var e body).rec' (motive:=motive) ret var
     = var e body (body.rec' ret var) :=
@@ -417,41 +422,41 @@ theorem Com.recAux'_eq {motive : ∀ {Γ eff t}, Com d Γ eff t → Sort u} :
 --       the type of `motive`
 @[elab_as_elim]
 def Com.recPure {motive : ∀ {Γ t}, Com d Γ .pure t → Sort u}
-    (ret : ∀ {Γ t}, (v : Var Γ t) → motive (Com.ret v))
-    (var : ∀ {Γ} {t u : d.Ty},
-      (e : Expr d Γ .pure t) → (body : Com d (Ctxt.snoc Γ t) .pure u) →
+    (ret : ∀ {Γ : Ctxt _} {ts}, (vs : HVector Γ.Var ts) → motive (Com.ret vs))
+    (var : ∀ {Γ Δ} {ts},
+      (e : Expr d Γ .pure Δ) → (body : Com d Δ .pure ts) →
         motive body → motive (Com.var e body))
     {Γ t} (com : Com d Γ .pure t) : motive com :=
   let motive {_Γ eff _t} (com) := match eff with
     | EffectKind.pure => motive com
     | EffectKind.impure => PUnit
-  let ret {Γ eff t} (v : Var Γ t) : @motive Γ eff t (Com.ret v) := match eff with
-    | .pure => ret v
+  let ret {Γ eff t} (vs : _) : @motive Γ eff t (Com.ret vs) := match eff with
+    | .pure => ret vs
     | .impure => ⟨⟩
-  let var {Γ t u} {eff} (e : Expr d Γ eff t) (body : Com d (Γ.snoc t) eff u) :
+  let var {Γ Δ u} {eff} (e : Expr d Γ eff Δ) (body : Com d Δ eff u) :
       motive body → motive (body.var e) :=
     fun r => match eff with
       | .pure => var _ _ r
       | .impure => ⟨⟩
   com.rec' (motive := @motive) ret var
 
-def Expr.op {Γ : Ctxt d.Ty} {eff : EffectKind} {ty : d.Ty} (e : Expr d Γ eff ty) : d.Op :=
+def Expr.op {Γ : Ctxt d.Ty} {eff : EffectKind} {Δ} (e : Expr d Γ eff Δ) : d.Op :=
   Expr.casesOn e (fun op _ _ _ _ => op)
 
-theorem Expr.eff_le {Γ : Ctxt d.Ty} {ty : d.Ty} (e : Expr d Γ eff ty) :
+theorem Expr.eff_le {Γ Δ : Ctxt d.Ty} (e : Expr d Γ eff Δ) :
   DialectSignature.effectKind e.op ≤ eff :=
   Expr.casesOn e (fun _ _ eff_le _ _ => eff_le)
 
-theorem Expr.ty_eq {Γ : Ctxt d.Ty} {ty : d.Ty} (e : Expr d Γ eff ty) :
-    ty = DialectSignature.outTy e.op :=
+theorem Expr.ty_eq {Γ Δ : Ctxt d.Ty} (e : Expr d Γ eff Δ) :
+    Δ = Γ ++ DialectSignature.returnTypes e.op :=
   Expr.casesOn e (fun _ ty_eq _ _ _ => ty_eq)
 
-def Expr.args {Γ : Ctxt d.Ty} {ty : d.Ty} (e : Expr d Γ eff ty) :
+def Expr.args {Γ Δ : Ctxt d.Ty} (e : Expr d Γ eff Δ) :
     HVector (Var Γ) (DialectSignature.sig e.op) :=
   Expr.casesOn e (fun _ _ _ args _ => args)
 
-def Expr.regArgs {Γ : Ctxt d.Ty} {ty : d.Ty} (e : Expr d Γ eff ty) :
-    HVector (fun t : Ctxt d.Ty × d.Ty => Com d t.1 .impure t.2) (DialectSignature.regSig e.op) :=
+def Expr.regArgs {Γ Δ : Ctxt d.Ty} (e : Expr d Γ eff Δ) :
+    HVector (fun t : Ctxt d.Ty × List d.Ty => Com d t.1 .impure t.2) (DialectSignature.regSig e.op) :=
   Expr.casesOn e (fun _ _ _ _ regArgs => regArgs)
 
 /-! Projection equations for `Expr` -/
